ExtParser/Parsing.lean
@@ -7,7 +7,7 @@ namespace Parsing
     | skip : TrueToGrammar (.skip s e G) Pexp G
     | ε : TrueToGrammar (.ε s e) Pexp .ε
     | any : TrueToGrammar (.any s e x) Pexp .any
-    | terminal : TrueToGrammar (.terminal s e a x) Pexp (.terminal x)
+    | terminal : TrueToGrammar (.terminal s e a x) Pexp (.terminal a)
     | nonTerminal : TrueToGrammar T Pexp (Pexp.f A) → TrueToGrammar (.nonTerminal s e A T) Pexp (.nonTerminal A)
     | seq : TrueToGrammar T1 Pexp e1 → TrueToGrammar T2 Pexp e2 → TrueToGrammar (.seq s e T1 T2) Pexp (.seq e1 e2)
     | prior : TrueToGrammar T1 Pexp e1 → TrueToGrammar T2 Pexp e2 → TrueToGrammar (.prior s e T1 T2) Pexp (.prior e1 e2)
@@ -88,7 +88,7 @@ namespace Parsing
                   exact Nat.lt_of_lt_of_le (Nat.succ_lt_succ g) hend;
                 }
             }
-          | .any (Or.inr (.any h)) =>
+          | .any (Or.inr (.any h _)) =>
             {
               rw [h] at hstart;
               apply absurd hstart;
@@ -125,7 +125,7 @@ namespace Parsing
                   exact Nat.lt_of_lt_of_le (Nat.succ_lt_succ g) hend;
                 }
             }
-          | .terminal (Or.inr (.terminal_empty h)) =>
+          | .terminal (Or.inr (.terminal_empty h _)) =>
             {
               rw [h] at hstart;
               apply absurd hstart;
@@ -237,5 +237,533 @@ namespace Parsing
               apply absurd g (Nat.lt_irrefl e);
             }
         }
+
+
+  theorem AST.unique_tree : ∀ {T1 T2 : AST n b} {inp : Input b} {G : PEG n} {Pexp : GProd n}, 
+                            AST.TrueToInput T1 inp → AST.TrueToInput T2 inp → 
+                            AST.TrueToGrammar T1 Pexp G → AST.TrueToGrammar T2 Pexp G → 
+                            T1.start = T2.start → T1 = T2 := by
+    intro (.mk T1 valid_T1 wf_T1) (.mk T2 valid_T2 wf_T2) inp G Pexp hi1 hi2 hg1 hg2 hstart;
+    cases T1 with
+    | skip _ _ _ => cases wf_T1;
+    | ε s1 e1 => cases T2 with
+      | skip _ _ _ => cases wf_T2;
+      | ε s2 e2 =>
+      {
+        simp [AST.start, PreAST.start] at hstart; simp [hstart];
+        match wf_T1, wf_T2 with
+        | .ε (Or.inl (.ε h1)), .ε (Or.inl (.ε h2)) => rw [←h1, hstart, h2];
+      }
+      | _ => cases hg1; cases hg2;
+    | any s1 e1 x1 => cases T2 with
+      | skip _ _ _ => cases wf_T2;
+      | any s2 e2 x2 =>
+      {
+        simp [AST.start, PreAST.start] at hstart; simp [hstart];
+        have hx : x1 = x2 := by
+          {
+            simp [hstart] at hi1;
+            cases hi1; cases hi2;
+            apply Eq.trans; apply Eq.symm; assumption; assumption;
+          }
+        simp [hx];
+        match wf_T1, wf_T2 with
+        | .any (Or.inl (.any h1)), .any (Or.inl (.any h2)) =>
+          {
+            simp [hstart] at h1;
+            exact Eq.trans (Eq.symm h1) h2;
+          }
+        | .any (Or.inl (.any h1)), .any (Or.inr (.any h2 hb2)) =>
+          {
+            rw [←h2, ←hstart, Fin.IsMax] at hb2;
+            contradiction;
+          }
+        | .any (Or.inr (.any h1 hb1)), .any (Or.inl (.any h2)) =>
+          {
+            rw [←h1, hstart, Fin.IsMax] at hb1;
+            contradiction;
+          }
+        | .any (Or.inr (.any h1 hb1)), .any (Or.inr (.any h2 hb2)) =>
+          {
+            rw [←h1, hstart, h2];
+          }
+      }
+      | _ => cases hg1; cases hg2;
+    | terminal s1 e1 a1 x1 => cases T2 with
+      | skip _ _ _ => cases wf_T2;
+      | terminal s2 e2 a2 x2 =>
+      {
+        simp [AST.start, PreAST.start] at hstart; simp [hstart];
+        have hx : x1 = x2 := by
+          {
+            simp [hstart] at hi1;
+            cases hi1; cases hi2;
+            apply Eq.trans; apply Eq.symm; assumption; assumption;
+          }
+        simp [hx];
+        cases hg1; cases hg2; simp;
+        match wf_T1, wf_T2 with
+        | .terminal (Or.inl (.terminal h1 g1)), .terminal (Or.inl (.terminal h2 g2)) =>
+          {
+            simp [g1, ←g2];
+            apply Fin.eq_of_val_eq;
+            simp [←Fin.val_eq_of_eq h1, ←Fin.val_eq_of_eq h2, Fin.inbound_succ];
+            exact Fin.val_eq_of_eq hstart;
+          }
+        | .terminal (Or.inl (.terminal h1 g1)), .terminal (Or.inr (.terminal_mismatch h2 g2)) =>
+          {
+            rw [hx] at g1;
+            contradiction;
+          }
+        | .terminal (Or.inl (.terminal h1 g1)), .terminal (Or.inr (.terminal_empty h2 hb2)) =>
+          {
+            simp [←h2, ←hstart, Fin.IsMax] at hb2;
+            contradiction;
+          }
+        | .terminal (Or.inr (.terminal_mismatch h1 g1)), .terminal (Or.inl (.terminal h2 g2)) =>
+          {
+            rw [hx] at g1; contradiction;
+          }
+        | .terminal (Or.inr (.terminal_mismatch h1 g1)), .terminal (Or.inr (.terminal_mismatch h2 g2)) =>
+          {
+            apply Fin.eq_of_val_eq;
+            simp [←Fin.val_eq_of_eq h1, ←Fin.val_eq_of_eq h2, Fin.inbound_succ];
+            exact Fin.val_eq_of_eq hstart;
+          }
+        | .terminal (Or.inr (.terminal_mismatch h1 g1)), .terminal (Or.inr (.terminal_empty h2 hb2)) =>
+          {
+            simp [←h2, ←hstart, Fin.IsMax] at hb2;
+            contradiction;
+          }
+        | .terminal (Or.inr (.terminal_empty h1 hb1)), .terminal (Or.inl (.terminal h2 g2)) =>
+          {
+            simp [←h1, hstart, Fin.IsMax] at hb1;
+            contradiction;
+          }
+        | .terminal (Or.inr (.terminal_empty h1 hb1)), .terminal (Or.inr (.terminal_mismatch h2 g2)) =>
+          {
+            simp [←h1, hstart, Fin.IsMax] at hb1;
+            contradiction;
+          }
+        | .terminal (Or.inr (.terminal_empty h1 hb1)), .terminal (Or.inr (.terminal_empty h2 hb2)) =>
+          {
+            simp [←h1, hstart, h2];
+          }
+      }
+      | _ => cases hg1; cases hg2;
+    | nonTerminal s1 e1 A1 T1 => cases T2 with
+      | skip _ _ _ => cases wf_T2;
+      | nonTerminal s2 e2 A2 T2 =>
+      {
+        simp [AST.start, PreAST.start] at hstart; simp [hstart];
+        match wf_T1, wf_T2, valid_T1, valid_T2 with
+        | .nonTerminal hss1 hee1 hwfT1, .nonTerminal hss2 hee2 hwfT2, .nonTerminal hvT1 _ , .nonTerminal hvT2 _ =>
+          {
+            cases hi1; cases hi2; cases hg1; cases hg2;
+            have _ : (AST.mk T1 hvT1 hwfT1).size < (AST.mk (.nonTerminal s1 e1 A1 T1) valid_T1 wf_T1).size := by
+            {
+              simp [AST.size, PreAST.size]; apply Nat.lt_succ_self;
+            }
+            have g : AST.mk T1 hvT1 hwfT1 = AST.mk T2 hvT2 hwfT2 := by
+            {
+              apply unique_tree;
+              assumption;
+              assumption;
+              assumption;
+              assumption;
+              simp [AST.start, ←hss1, ←hss2, hstart];
+            }
+            cases g;
+            simp [hee1, hee2];
+          }
+      }
+      | _ => cases hg1; cases hg2;
+    | seq s1 e1 T11 T21 => cases T2 with
+      | skip _ _ _ => cases wf_T2;
+      | seq s2 e2 T12 T22 =>
+      {
+        simp [AST.start, PreAST.start] at hstart; simp [hstart];
+        match wf_T1, wf_T2 with
+        | .seq_F hss11 he11s21 hee21 hs21e21 hwf11 hf11 hskip21, .seq_F hss12 he12s22 hee22 hs22e22 hwf12 hf12 hskip22 =>
+          {
+            cases hi1; cases hi2;
+            match hg1, hg2, valid_T1, valid_T2 with
+            | .seq hg11 hg21, .seq hg12 hg22, .seq hv11 _ _, .seq hv12 _ _ =>
+            {
+              have _ : (AST.mk T11 hv11 hwf11).size < (AST.mk (.seq s1 e1 T11 T21) valid_T1 wf_T1).size := by
+              {
+                simp [AST.size, PreAST.size]; rw [←Nat.add_zero (PreAST.size T11), Nat.add_assoc (PreAST.size T11 + 0)]; apply Nat.add_lt_add_left; apply Nat.zero_lt_succ;
+              }
+              have g1 : AST.mk T11 hv11 hwf11 = AST.mk T12 hv12 hwf12 := by
+              {
+                apply unique_tree;
+                assumption;
+                assumption;
+                assumption;
+                assumption;
+                simp [AST.start, ←hss11, ←hss12, hstart];
+              }
+              cases g1; simp;
+              cases hskip21; cases hskip22;
+              cases hg21; cases hg22;
+              simp [PreAST.start, PreAST.end] at hs21e21 hee21 hs22e22 hee22;
+              simp [PreAST.start] at he11s21 he12s22;
+              simp [hee21, hee22, ←he11s21, ←he12s22, ←hs21e21, ←hs22e22];
+            }
+          }
+        | .seq_F hss11 he11s21 hee21 hs21e21 hwf11 hf11 _, .seq_S hss12 he12s22 hee22 hwf12 hs12 _ =>
+          {
+            cases hi1; cases hi2;
+            match hg1, hg2, valid_T1, valid_T2 with
+            | .seq hg11 hg21, .seq hg12 hg22, .seq hv11 _ _, .seq hv12 _ _ =>
+            {
+              have _ : (AST.mk T11 hv11 hwf11).size < (AST.mk (.seq s1 e1 T11 T21) valid_T1 wf_T1).size := by
+              {
+                simp [AST.size, PreAST.size]; rw [←Nat.add_zero (PreAST.size T11), Nat.add_assoc (PreAST.size T11 + 0)]; apply Nat.add_lt_add_left; apply Nat.zero_lt_succ;
+              }
+              have g1 : AST.mk T11 hv11 hwf11 = AST.mk T12 hv12 hwf12 := by
+              {
+                apply unique_tree;
+                assumption;
+                assumption;
+                assumption;
+                assumption;
+                simp [AST.start, ←hss11, ←hss12, hstart];
+              }
+              cases g1; simp;
+              exact absurd hf11 (hs12.ne_failure (by assumption));
+            }
+          }
+        | .seq_S hss11 he11s21 hee21 hwf11 hs11 _, .seq_F hss12 he12s22 hee22 hs22e22 hwf12 hf12 _ =>
+          {
+            cases hi1; cases hi2;
+            match hg1, hg2, valid_T1, valid_T2 with
+            | .seq hg11 hg21, .seq hg12 hg22, .seq hv11 _ _, .seq hv12 _ _ =>
+            {
+              have _ : (AST.mk T11 hv11 hwf11).size < (AST.mk (.seq s1 e1 T11 T21) valid_T1 wf_T1).size := by
+              {
+                simp [AST.size, PreAST.size]; rw [←Nat.add_zero (PreAST.size T11), Nat.add_assoc (PreAST.size T11 + 0)]; apply Nat.add_lt_add_left; apply Nat.zero_lt_succ;
+              }
+              have g1 : AST.mk T11 hv11 hwf11 = AST.mk T12 hv12 hwf12 := by
+              {
+                apply unique_tree;
+                assumption;
+                assumption;
+                assumption;
+                assumption;
+                simp [AST.start, ←hss11, ←hss12, hstart];
+              }
+              cases g1; simp;
+              exact absurd hs11 (hf12.ne_success (by assumption));
+            }
+          }
+        | .seq_S hss11 he11s21 hee21 hwf11 hs11 hwf21, .seq_S hss12 he12s22 hee22 hwf12 hs12 hwf22 =>
+          {
+            cases hi1; cases hi2;
+            match hg1, hg2, valid_T1, valid_T2 with
+            | .seq hg11 hg21, .seq hg12 hg22, .seq hv11 hv21 _, .seq hv12 hv22 _ =>
+            {
+              have _ : (AST.mk T11 hv11 hwf11).size < (AST.mk (.seq s1 e1 T11 T21) valid_T1 wf_T1).size := by
+              {
+                simp [AST.size, PreAST.size]; rw [←Nat.add_zero (PreAST.size T11), Nat.add_assoc (PreAST.size T11 + 0)]; apply Nat.add_lt_add_left; apply Nat.zero_lt_succ;
+              }
+              have g1 : AST.mk T11 hv11 hwf11 = AST.mk T12 hv12 hwf12 := by
+              {
+                apply unique_tree;
+                assumption;
+                assumption;
+                assumption;
+                assumption;
+                simp [AST.start, ←hss11, ←hss12, hstart];
+              }
+              cases g1; simp;
+              have _ : (AST.mk T21 hv21 hwf21).size < (AST.mk (.seq s1 e1 T11 T21) valid_T1 wf_T1).size := by
+              {
+                simp [AST.size, PreAST.size]; rw [Nat.add_comm (PreAST.size T11), ←Nat.add_zero (PreAST.size T21), Nat.add_assoc (PreAST.size T21 + 0)];
+                apply Nat.add_lt_add_left; apply Nat.zero_lt_succ;
+              }
+              have g2 : AST.mk T21 hv21 hwf21 = AST.mk T22 hv22 hwf22 := by
+              {
+                apply unique_tree;
+                assumption;
+                assumption;
+                assumption;
+                assumption;
+                simp [AST.start, ←he11s21, ←he12s22];
+              }
+              cases g2; simp;
+              simp [hee21, hee22];
+            }
+          }
+      }
+      | _ => cases hg1; cases hg2;
+    | prior s1 e1 T11 T21 => cases T2 with
+      | skip _ _ _ => cases wf_T2;
+      | prior s2 e2 T12 T22 =>
+      {
+        simp [AST.start, PreAST.start] at hstart; simp [hstart];
+        match wf_T1, wf_T2 with
+        | .prior_F hss11 hss21 hee21 hwf11 hf11 hwf21, .prior_F hss12 hss22 hee22 hwf12 hf12 hwf22 =>
+          {
+            cases hi1; cases hi2;
+            match hg1, hg2, valid_T1, valid_T2 with
+            | .prior hg11 hg21, .prior hg12 hg22, .prior hv11 hv21 _, .prior hv12 hv22 _ =>
+            {
+              have _ : (AST.mk T11 hv11 hwf11).size < (AST.mk (.prior s1 e1 T11 T21) valid_T1 wf_T1).size := by
+              {
+                simp [AST.size, PreAST.size]; rw [←Nat.add_zero (PreAST.size T11), Nat.add_assoc (PreAST.size T11 + 0)]; apply Nat.add_lt_add_left; apply Nat.zero_lt_succ;
+              }
+              have g1 : AST.mk T11 hv11 hwf11 = AST.mk T12 hv12 hwf12 := by
+              {
+                apply unique_tree;
+                assumption;
+                assumption;
+                assumption;
+                assumption;
+                simp [AST.start, ←hss11, ←hss12, hstart];
+              }
+              have _ : (AST.mk T21 hv21 hwf21).size < (AST.mk (.prior s1 e1 T11 T21) valid_T1 wf_T1).size := by
+              {
+                simp [AST.size, PreAST.size]; rw [Nat.add_comm (PreAST.size T11), ←Nat.add_zero (PreAST.size T21), Nat.add_assoc (PreAST.size T21 + 0)];
+                apply Nat.add_lt_add_left; apply Nat.zero_lt_succ;
+              }
+              have g2 : AST.mk T21 hv21 hwf21 = AST.mk T22 hv22 hwf22 := by
+              {
+                apply unique_tree;
+                assumption;
+                assumption;
+                assumption;
+                assumption;
+                simp [AST.start, ←hss21, ←hss22, hstart];
+              }
+              cases g1; cases g2; simp;
+              simp [hee21, hee22];
+            }
+          }
+        | .prior_F hss11 hss21 hee21 hwf11 hf11 hwf21, .prior_S hss12 hss22 hse22 hee12 hwf12 hs12 hskip22 =>
+          {
+            cases hi1; cases hi2;
+            match hg1, hg2, valid_T1, valid_T2 with
+            | .prior hg11 hg21, .prior hg12 hg22, .prior hv11 hv21 _, .prior hv12 hv22 _ =>
+            {
+              have _ : (AST.mk T11 hv11 hwf11).size < (AST.mk (.prior s1 e1 T11 T21) valid_T1 wf_T1).size := by
+              {
+                simp [AST.size, PreAST.size]; rw [←Nat.add_zero (PreAST.size T11), Nat.add_assoc (PreAST.size T11 + 0)]; apply Nat.add_lt_add_left; apply Nat.zero_lt_succ;
+              }
+              have g1 : AST.mk T11 hv11 hwf11 = AST.mk T12 hv12 hwf12 := by
+              {
+                apply unique_tree;
+                assumption;
+                assumption;
+                assumption;
+                assumption;
+                simp [AST.start, ←hss11, ←hss12, hstart];
+              }
+              cases g1; simp;
+              exact absurd hf11 (hs12.ne_failure (by assumption));
+            }
+          }
+        | .prior_S hss11 hss21 hse21 hee11 hwf11 hs11 hskip21, .prior_F hss12 hss22 hee22 hwf12 hf12 hwf22 =>
+          {
+            cases hi1; cases hi2;
+            match hg1, hg2, valid_T1, valid_T2 with
+            | .prior hg11 hg21, .prior hg12 hg22, .prior hv11 hv21 _, .prior hv12 hv22 _ =>
+            {
+              have _ : (AST.mk T11 hv11 hwf11).size < (AST.mk (.prior s1 e1 T11 T21) valid_T1 wf_T1).size := by
+              {
+                simp [AST.size, PreAST.size]; rw [←Nat.add_zero (PreAST.size T11), Nat.add_assoc (PreAST.size T11 + 0)]; apply Nat.add_lt_add_left; apply Nat.zero_lt_succ;
+              }
+              have g1 : AST.mk T11 hv11 hwf11 = AST.mk T12 hv12 hwf12 := by
+              {
+                apply unique_tree;
+                assumption;
+                assumption;
+                assumption;
+                assumption;
+                simp [AST.start, ←hss11, ←hss12, hstart];
+              }
+              cases g1; simp;
+              exact absurd hs11 (hf12.ne_success (by assumption));
+            }
+          }
+        | .prior_S hss11 hss21 hse21 hee11 hwf11 hs11 hskip21, .prior_S hss12 hss22 hse22 hee12 hwf12 hs12 hskip22 =>
+          {
+            cases hi1; cases hi2;
+            match hg1, hg2, valid_T1, valid_T2 with
+            | .prior hg11 hg21, .prior hg12 hg22, .prior hv11 hv21 _, .prior hv12 hv22 _ =>
+            {
+              have _ : (AST.mk T11 hv11 hwf11).size < (AST.mk (.prior s1 e1 T11 T21) valid_T1 wf_T1).size := by
+              {
+                simp [AST.size, PreAST.size]; rw [←Nat.add_zero (PreAST.size T11), Nat.add_assoc (PreAST.size T11 + 0)]; apply Nat.add_lt_add_left; apply Nat.zero_lt_succ;
+              }
+              have g1 : AST.mk T11 hv11 hwf11 = AST.mk T12 hv12 hwf12 := by
+              {
+                apply unique_tree;
+                assumption;
+                assumption;
+                assumption;
+                assumption;
+                simp [AST.start, ←hss11, ←hss12, hstart];
+              }
+              cases g1; simp;
+              cases hskip21; cases hskip22;
+              cases hg21; cases hg22;
+              simp [PreAST.start] at hss21 hss22;
+              simp [PreAST.end] at hse21 hse22;
+              simp [hee11, hee12, ←hss21, ←hse21, ←hss22, ←hse22, hstart];
+            }
+          }
+      }
+      | _ => cases hg1; cases hg2;
+    | star s1 e1 T01 TS1 => cases T2 with
+      | skip _ _ _ => cases wf_T2;
+      | star s2 e2 T02 TS2 =>
+      {
+        simp [AST.start, PreAST.start] at hstart; simp [hstart];
+        match wf_T1, wf_T2 with
+        | .star_F hss01 he01sS1 hsS1eS1 hse1 hwf01 hf01 hskipS1, .star_F hss02 he02sS2 hsS2eS2 hse2 hwf02 hf02 hskipS2 =>
+          {
+            cases hi1; cases hi2;
+            match hg1, hg2, valid_T1, valid_T2 with
+            | .star hg01 hgS1, .star hg02 hgS2, .star hv01 hvS1 _ _, .star hv02 hvS2 _ _ =>
+            {
+              have _ : (AST.mk T01 hv01 hwf01).size < (AST.mk (.star s1 e1 T01 TS1) valid_T1 wf_T1).size := by
+              {
+                simp [AST.size, PreAST.size]; rw [←Nat.add_zero (PreAST.size T01), Nat.add_assoc (PreAST.size T01 + 0)]; apply Nat.add_lt_add_left; apply Nat.zero_lt_succ;
+              }
+              have g1 : AST.mk T01 hv01 hwf01 = AST.mk T02 hv02 hwf02 := by
+              {
+                apply unique_tree;
+                assumption;
+                assumption;
+                assumption;
+                assumption;
+                simp [AST.start, ←hss01, ←hss02, hstart];
+              }
+              cases g1; simp;
+              cases hskipS1; cases hskipS2;
+              cases hgS1; cases hgS2;
+              simp [PreAST.start, PreAST.end] at hsS1eS1 hsS2eS2;
+              simp [PreAST.start] at he01sS1 he02sS2;
+              simp [←hse1, ←hse2, ←hsS1eS1, ←hsS2eS2, ←he01sS1, ←he02sS2, hstart];
+            }
+          }
+        | .star_F hss01 he01sS1 hsS1eS1 hse1 hwf01 hf01 hskipS1, .star_S hss02 he02sS2 heeS2 hwf02 hs02 hwfS2 =>
+          {
+            cases hi1; cases hi2;
+            match hg1, hg2, valid_T1, valid_T2 with
+            | .star hg01 hgS1, .star hg02 hgS2, .star hv01 hvS1 _ _, .star hv02 hvS2 _ _ =>
+            {
+              have _ : (AST.mk T01 hv01 hwf01).size < (AST.mk (.star s1 e1 T01 TS1) valid_T1 wf_T1).size := by
+              {
+                simp [AST.size, PreAST.size]; rw [←Nat.add_zero (PreAST.size T01), Nat.add_assoc (PreAST.size T01 + 0)]; apply Nat.add_lt_add_left; apply Nat.zero_lt_succ;
+              }
+              have g1 : AST.mk T01 hv01 hwf01 = AST.mk T02 hv02 hwf02 := by
+              {
+                apply unique_tree;
+                assumption;
+                assumption;
+                assumption;
+                assumption;
+                simp [AST.start, ←hss01, ←hss02, hstart];
+              }
+              cases g1; simp;
+              exact absurd hf01 (hs02.ne_failure (by assumption));
+            }
+          }
+        | .star_S hss01 he01sS1 heeS1 hwf01 hs01 hwfS1, .star_F hss02 he02sS2 hsS2eS2 hse2 hwf02 hf02 hskipS2 =>
+          {
+            cases hi1; cases hi2;
+            match hg1, hg2, valid_T1, valid_T2 with
+            | .star hg01 hgS1, .star hg02 hgS2, .star hv01 hvS1 _ _, .star hv02 hvS2 _ _ =>
+            {
+              have _ : (AST.mk T01 hv01 hwf01).size < (AST.mk (.star s1 e1 T01 TS1) valid_T1 wf_T1).size := by
+              {
+                simp [AST.size, PreAST.size]; rw [←Nat.add_zero (PreAST.size T01), Nat.add_assoc (PreAST.size T01 + 0)]; apply Nat.add_lt_add_left; apply Nat.zero_lt_succ;
+              }
+              have g1 : AST.mk T01 hv01 hwf01 = AST.mk T02 hv02 hwf02 := by
+              {
+                apply unique_tree;
+                assumption;
+                assumption;
+                assumption;
+                assumption;
+                simp [AST.start, ←hss01, ←hss02, hstart];
+              }
+              cases g1; simp;
+              exact absurd hs01 (hf02.ne_success (by assumption));
+            }
+          }
+        | .star_S hss01 he01sS1 heeS1 hwf01 hs01 hwfS1, .star_S hss02 he02sS2 heeS2 hwf02 hs02 hwfS2 =>
+          {
+            cases hi1; cases hi2;
+            match hg1, hg2, valid_T1, valid_T2 with
+            | .star hg01 hgS1, .star hg02 hgS2, .star hv01 hvS1 _ _, .star hv02 hvS2 _ _ =>
+            {
+              have _ : (AST.mk T01 hv01 hwf01).size < (AST.mk (.star s1 e1 T01 TS1) valid_T1 wf_T1).size := by
+              {
+                simp [AST.size, PreAST.size]; rw [←Nat.add_zero (PreAST.size T01), Nat.add_assoc (PreAST.size T01 + 0)]; apply Nat.add_lt_add_left; apply Nat.zero_lt_succ;
+              }
+              have g1 : AST.mk T01 hv01 hwf01 = AST.mk T02 hv02 hwf02 := by
+              {
+                apply unique_tree;
+                assumption;
+                assumption;
+                assumption;
+                assumption;
+                simp [AST.start, ←hss01, ←hss02, hstart];
+              }
+              cases g1; simp;
+              have _ : (AST.mk TS1 hvS1 hwfS1).size < (AST.mk (.star s1 e1 T01 TS1) valid_T1 wf_T1).size := by
+              {
+                simp [AST.size, PreAST.size]; rw [Nat.add_comm (PreAST.size T01), ←Nat.add_zero (PreAST.size TS1), Nat.add_assoc (PreAST.size TS1 + 0)];
+                apply Nat.add_lt_add_left; apply Nat.zero_lt_succ;
+              }
+              have g2 : AST.mk TS1 hvS1 hwfS1 = AST.mk TS2 hvS2 hwfS2 := by
+              {
+                apply unique_tree;
+                assumption;
+                assumption;
+                assumption;
+                assumption;
+                simp [AST.start, ←he01sS1, ←he02sS2];
+              }
+              cases g2; simp;
+              simp [heeS1, heeS2];
+            }
+          }
+      }
+      | _ => cases hg1; cases hg2;
+    | notP s1 e1 T1 => cases T2 with
+      | skip _ _ _ => cases wf_T2;
+      | notP s2 e2 T2 =>
+      {
+        simp [AST.start, PreAST.start] at hstart; simp [hstart];
+        match wf_T1, wf_T2, valid_T1, valid_T2 with
+        | .notP hse1 hssT1 hwfT1, .notP hse2 hssT2 hwfT2, .notP hv1 _, .notP hv2 _ =>
+        {
+          have _ : (AST.mk T1 hv1 hwfT1).size < (AST.mk (.notP s1 e1 T1) valid_T1 wf_T1).size := by
+          {
+            simp [AST.size, PreAST.size]; apply Nat.lt_succ_self;
+          }
+          have g : AST.mk T1 hv1 hwfT1 = AST.mk T2 hv2 hwfT2 := by
+          {
+            cases hi1; cases hi2; cases hg1; cases hg2;
+            apply unique_tree;
+            assumption;
+            assumption;
+            assumption;
+            assumption;
+            simp [AST.start, ←hssT1, ←hssT2, hstart];
+          }
+          cases g; simp;
+          simp [←hse1, ←hse2, hstart];
+        }
+      }
+      | _ => cases hg1; cases hg2;
+  termination_by AST.unique_tree _ _ T1 => T1.size
+  decreasing_by sorry
+
+
 
 end Parsing
